src/test/dafny/IntTests.dfy
@@ -1,402 +1,409 @@
 include "../../dafny/util/int.dfy"
 include "utils.dfy"
 
-import opened Int
+module IntTests {
+    import opened Int
+    import opened Utils
+    import opened U16
+    import opened U256
+    import opened I256
+    import opened Word
 
-// Various tests for roundup
-method {:test} RoundUpTests() {
-    Assert(() => RoundUp(2,16) == 16);
-    Assert(() => RoundUp(16,16) == 16);
-    Assert(() => RoundUp(17,16) == 32);
-    Assert(() => RoundUp(31,16) == 32);
-    Assert(() => RoundUp(32,16) == 32);
-    Assert(() => RoundUp(33,16) == 48);
-}
+    // Various tests for roundup
+    method {:test} RoundUpTests() {
+        Assert(() => RoundUp(2,16) == 16);
+        Assert(() => RoundUp(16,16) == 16);
+        Assert(() => RoundUp(17,16) == 32);
+        Assert(() => RoundUp(31,16) == 32);
+        Assert(() => RoundUp(32,16) == 32);
+        Assert(() => RoundUp(33,16) == 48);
+    }
 
-// Various sanity tests for division.
-method {:test} DivTests() {
-    // pos-pos
-    Assert(()=> Div(6,2) == 3);
-    Assert(()=> Div(6,3) == 2);
-    Assert(()=> Div(6,4) == 1);
-    Assert(()=> Div(9,4) == 2);
-    // neg-pos
-    Assert(()=> Div(-6,2) == -3);
-    Assert(()=> Div(-6,3) == -2);
-    Assert(()=> Div(-6,4) == -1);
-    Assert(()=> Div(-9,4) == -2);
-    // pos-neg
-    Assert(()=> Div(6,-2) == -3);
-    Assert(()=> Div(6,-3) == -2);
-    Assert(()=> Div(6,-4) == -1);
-    Assert(()=> Div(9,-4) == -2);
-    // neg-neg
-    Assert(()=> Div(-6,-2) == 3);
-    Assert(()=> Div(-6,-3) == 2);
-    Assert(()=> Div(-6,-4) == 1);
-    Assert(()=> Div(-9,-4) == 2);
-    // Misc
-    Assert(()=> Div(-1,1) == -1);
-}
+    // Various sanity tests for division.
+    method {:test} DivTests() {
+        // pos-pos
+        Assert(()=> Int.Div(6,2) == 3);
+        Assert(()=> Int.Div(6,3) == 2);
+        Assert(()=> Int.Div(6,4) == 1);
+        Assert(()=> Int.Div(9,4) == 2);
+        // neg-pos
+        Assert(()=> Int.Div(-6,2) == -3);
+        Assert(()=> Int.Div(-6,3) == -2);
+        Assert(()=> Int.Div(-6,4) == -1);
+        Assert(()=> Int.Div(-9,4) == -2);
+        // pos-neg
+        Assert(()=> Int.Div(6,-2) == -3);
+        Assert(()=> Int.Div(6,-3) == -2);
+        Assert(()=> Int.Div(6,-4) == -1);
+        Assert(()=> Int.Div(9,-4) == -2);
+        // neg-neg
+        Assert(()=> Int.Div(-6,-2) == 3);
+        Assert(()=> Int.Div(-6,-3) == 2);
+        Assert(()=> Int.Div(-6,-4) == 1);
+        Assert(()=> Int.Div(-9,-4) == 2);
+        // Misc
+        Assert(()=> Int.Div(-1,1) == -1);
+    }
 
-// Various sanity tests for Remainder.
-method {:test} RemTests() {
-    // pos-pos
-    Assert(()=> Rem(6,2) == 0);
-    Assert(()=> Rem(6,3) == 0);
-    Assert(()=> Rem(6,4) == 2);
-    Assert(()=> Rem(9,4) == 1);
-    // neg-pos
-    Assert(()=> Rem(-6,2) == 0);
-    Assert(()=> Rem(-6,3) == 0);
-    Assert(()=> Rem(-6,4) == -2);
-    Assert(()=> Rem(-9,4) == -1);
-    // pos-neg
-    Assert(()=> Rem(6,-2) == 0);
-    Assert(()=> Rem(6,-3) == 0);
-    Assert(()=> Rem(6,-4) == 2);
-    Assert(()=> Rem(9,-4) == 1);
-    // neg-neg
-    Assert(()=> Rem(-6,-2) == 0);
-    Assert(()=> Rem(-6,-3) == 0);
-    Assert(()=> Rem(-6,-4) == -2);
-    Assert(()=> Rem(-9,-4) == -1);
-}
+    // Various sanity tests for Remainder.
+    method {:test} RemTests() {
+        // pos-pos
+        Assert(()=> Int.Rem(6,2) == 0);
+        Assert(()=> Int.Rem(6,3) == 0);
+        Assert(()=> Int.Rem(6,4) == 2);
+        Assert(()=> Int.Rem(9,4) == 1);
+        // neg-pos
+        Assert(()=> Int.Rem(-6,2) == 0);
+        Assert(()=> Int.Rem(-6,3) == 0);
+        Assert(()=> Int.Rem(-6,4) == -2);
+        Assert(()=> Int.Rem(-9,4) == -1);
+        // pos-neg
+        Assert(()=> Int.Rem(6,-2) == 0);
+        Assert(()=> Int.Rem(6,-3) == 0);
+        Assert(()=> Int.Rem(6,-4) == 2);
+        Assert(()=> Int.Rem(9,-4) == 1);
+        // neg-neg
+        Assert(()=> Int.Rem(-6,-2) == 0);
+        Assert(()=> Int.Rem(-6,-3) == 0);
+        Assert(()=> Int.Rem(-6,-4) == -2);
+        Assert(()=> Int.Rem(-9,-4) == -1);
+    }
 
- // Various sanity tests for exponentiation.
-method {:test} PowTests() {
-    Assert(()=> Pow(2,8) == TWO_8);
-    Assert(()=> Pow(2,15) == TWO_15);
-    Assert(()=> Pow(2,16) == TWO_16);
-    Assert(()=> Pow(2,24) == TWO_24);
-    Assert(()=> Pow(2,31) == TWO_31);
-    Assert(()=> Pow(2,32) == TWO_32);
-    Assert(()=> Pow(2,40) == TWO_40);
-    Assert(()=> Pow(2,48) == TWO_48);
-    Assert(()=> Pow(2,56) == TWO_56);
-    Assert(()=> Pow(2,63) == TWO_63);
-    Assert(()=> Pow(2,64) == TWO_64);
-    // NOTE:  I have to break the following ones up because Z3
-    // cannot handle it.
-    Assert(()=> Pow(2,63) * Pow(2,64) == TWO_127);
-    Assert(()=> Pow(2,64) * Pow(2,64) == TWO_128);
-    Assert(()=> Pow(2,64) * Pow(2,64) * Pow(2,64) * Pow(2,64) == TWO_256);
-    Assert(()=> (TWO_128 / TWO_64) == TWO_64);
-    Assert(()=> (TWO_256 / TWO_128) == TWO_128);
-}
+    // Various sanity tests for exponentiation.
+    method {:test} PowTests() {
+        Assert(()=> Pow(2,8) == TWO_8);
+        Assert(()=> Pow(2,15) == TWO_15);
+        Assert(()=> Pow(2,16) == TWO_16);
+        Assert(()=> Pow(2,24) == TWO_24);
+        Assert(()=> Pow(2,31) == TWO_31);
+        Assert(()=> Pow(2,32) == TWO_32);
+        Assert(()=> Pow(2,40) == TWO_40);
+        Assert(()=> Pow(2,48) == TWO_48);
+        Assert(()=> Pow(2,56) == TWO_56);
+        Assert(()=> Pow(2,63) == TWO_63);
+        Assert(()=> Pow(2,64) == TWO_64);
+        // NOTE:  I have to break the following ones up because Z3
+        // cannot handle it.
+        Assert(()=> Pow(2,63) * Pow(2,64) == TWO_127);
+        Assert(()=> Pow(2,64) * Pow(2,64) == TWO_128);
+        Assert(()=> Pow(2,64) * Pow(2,64) * Pow(2,64) * Pow(2,64) == TWO_256);
+        Assert(()=> (TWO_128 / TWO_64) == TWO_64);
+        Assert(()=> (TWO_256 / TWO_128) == TWO_128);
+    }
 
-method {:test} NthUint8Tests() {
-    Assert(()=> U16.NthUint8(0xde80,0) == 0xde);
-    Assert(()=> U16.NthUint8(0xde80,1) == 0x80);
-    // U32
-    Assert(()=> U32.NthUint16(0x1230de80,0) == 0x1230);
-    Assert(()=> U32.NthUint16(0x1230de80,1) == 0xde80);
-    // U64
-    Assert(()=> U64.NthUint32(0x00112233_44556677,0) == 0x00112233);
-    Assert(()=> U64.NthUint32(0x00112233_44556677,1) == 0x44556677);
-    // U128
-    Assert(()=> U128.NthUint64(0x0011223344556677_8899AABBCCDDEEFF,0) == 0x0011223344556677);
-    Assert(()=> U128.NthUint64(0x0011223344556677_8899AABBCCDDEEFF,1) == 0x8899AABBCCDDEEFF);
-    // U256
-    Assert(()=> U256.NthUint128(0x00112233445566778899AABBCCDDEEFF_FFEEDDCCBBAA99887766554433221100,0) == 0x00112233445566778899AABBCCDDEEFF);
-    Assert(()=> U256.NthUint128(0x00112233445566778899AABBCCDDEEFF_FFEEDDCCBBAA99887766554433221100,1) == 0xFFEEDDCCBBAA99887766554433221100);
-    Assert(()=> U256.NthUint8(0x000102030405060708090A0B0C0D0E0F_101112131415161718191A1B1C1D1E1F,00) == 0x00);
-    Assert(()=> U256.NthUint8(0x000102030405060708090A0B0C0D0E0F_101112131415161718191A1B1C1D1E1F,01) == 0x01);
-    Assert(()=> U256.NthUint8(0x000102030405060708090A0B0C0D0E0F_101112131415161718191A1B1C1D1E1F,02) == 0x02);
-    Assert(()=> U256.NthUint8(0x000102030405060708090A0B0C0D0E0F_101112131415161718191A1B1C1D1E1F,03) == 0x03);
-    Assert(()=> U256.NthUint8(0x000102030405060708090A0B0C0D0E0F_101112131415161718191A1B1C1D1E1F,04) == 0x04);
-    Assert(()=> U256.NthUint8(0x000102030405060708090A0B0C0D0E0F_101112131415161718191A1B1C1D1E1F,05) == 0x05);
-    Assert(()=> U256.NthUint8(0x000102030405060708090A0B0C0D0E0F_101112131415161718191A1B1C1D1E1F,06) == 0x06);
-    Assert(()=> U256.NthUint8(0x000102030405060708090A0B0C0D0E0F_101112131415161718191A1B1C1D1E1F,07) == 0x07);
-    Assert(()=> U256.NthUint8(0x000102030405060708090A0B0C0D0E0F_101112131415161718191A1B1C1D1E1F,08) == 0x08);
-    Assert(()=> U256.NthUint8(0x000102030405060708090A0B0C0D0E0F_101112131415161718191A1B1C1D1E1F,09) == 0x09);
-    Assert(()=> U256.NthUint8(0x000102030405060708090A0B0C0D0E0F_101112131415161718191A1B1C1D1E1F,10) == 0x0A);
-    Assert(()=> U256.NthUint8(0x000102030405060708090A0B0C0D0E0F_101112131415161718191A1B1C1D1E1F,11) == 0x0B);
-    Assert(()=> U256.NthUint8(0x000102030405060708090A0B0C0D0E0F_101112131415161718191A1B1C1D1E1F,12) == 0x0C);
-    Assert(()=> U256.NthUint8(0x000102030405060708090A0B0C0D0E0F_101112131415161718191A1B1C1D1E1F,13) == 0x0D);
-    Assert(()=> U256.NthUint8(0x000102030405060708090A0B0C0D0E0F_101112131415161718191A1B1C1D1E1F,14) == 0x0E);
-    Assert(()=> U256.NthUint8(0x000102030405060708090A0B0C0D0E0F_101112131415161718191A1B1C1D1E1F,15) == 0x0F);
-    Assert(()=> U256.NthUint8(0x000102030405060708090A0B0C0D0E0F_101112131415161718191A1B1C1D1E1F,16) == 0x10);
-    Assert(()=> U256.NthUint8(0x000102030405060708090A0B0C0D0E0F_101112131415161718191A1B1C1D1E1F,17) == 0x11);
-    Assert(()=> U256.NthUint8(0x000102030405060708090A0B0C0D0E0F_101112131415161718191A1B1C1D1E1F,18) == 0x12);
-    Assert(()=> U256.NthUint8(0x000102030405060708090A0B0C0D0E0F_101112131415161718191A1B1C1D1E1F,19) == 0x13);
-    Assert(()=> U256.NthUint8(0x000102030405060708090A0B0C0D0E0F_101112131415161718191A1B1C1D1E1F,20) == 0x14);
-    Assert(()=> U256.NthUint8(0x000102030405060708090A0B0C0D0E0F_101112131415161718191A1B1C1D1E1F,21) == 0x15);
-    Assert(()=> U256.NthUint8(0x000102030405060708090A0B0C0D0E0F_101112131415161718191A1B1C1D1E1F,22) == 0x16);
-    Assert(()=> U256.NthUint8(0x000102030405060708090A0B0C0D0E0F_101112131415161718191A1B1C1D1E1F,23) == 0x17);
-    Assert(()=> U256.NthUint8(0x000102030405060708090A0B0C0D0E0F_101112131415161718191A1B1C1D1E1F,24) == 0x18);
-    Assert(()=> U256.NthUint8(0x000102030405060708090A0B0C0D0E0F_101112131415161718191A1B1C1D1E1F,25) == 0x19);
-    Assert(()=> U256.NthUint8(0x000102030405060708090A0B0C0D0E0F_101112131415161718191A1B1C1D1E1F,26) == 0x1A);
-    Assert(()=> U256.NthUint8(0x000102030405060708090A0B0C0D0E0F_101112131415161718191A1B1C1D1E1F,27) == 0x1B);
-    Assert(()=> U256.NthUint8(0x000102030405060708090A0B0C0D0E0F_101112131415161718191A1B1C1D1E1F,28) == 0x1C);
-    Assert(()=> U256.NthUint8(0x000102030405060708090A0B0C0D0E0F_101112131415161718191A1B1C1D1E1F,29) == 0x1D);
-    Assert(()=> U256.NthUint8(0x000102030405060708090A0B0C0D0E0F_101112131415161718191A1B1C1D1E1F,30) == 0x1E);
-    Assert(()=> U256.NthUint8(0x000102030405060708090A0B0C0D0E0F_101112131415161718191A1B1C1D1E1F,31) == 0x1F);
-}
+    method {:test} NthUint8Tests() {
+        Assert(()=> U16.NthUint8(0xde80,0) == 0xde);
+        Assert(()=> U16.NthUint8(0xde80,1) == 0x80);
+        // U32
+        Assert(()=> U32.NthUint16(0x1230de80,0) == 0x1230);
+        Assert(()=> U32.NthUint16(0x1230de80,1) == 0xde80);
+        // U64
+        Assert(()=> U64.NthUint32(0x00112233_44556677,0) == 0x00112233);
+        Assert(()=> U64.NthUint32(0x00112233_44556677,1) == 0x44556677);
+        // U128
+        Assert(()=> U128.NthUint64(0x0011223344556677_8899AABBCCDDEEFF,0) == 0x0011223344556677);
+        Assert(()=> U128.NthUint64(0x0011223344556677_8899AABBCCDDEEFF,1) == 0x8899AABBCCDDEEFF);
+        // U256
+        Assert(()=> U256.NthUint128(0x00112233445566778899AABBCCDDEEFF_FFEEDDCCBBAA99887766554433221100,0) == 0x00112233445566778899AABBCCDDEEFF);
+        Assert(()=> U256.NthUint128(0x00112233445566778899AABBCCDDEEFF_FFEEDDCCBBAA99887766554433221100,1) == 0xFFEEDDCCBBAA99887766554433221100);
+        Assert(()=> U256.NthUint8(0x000102030405060708090A0B0C0D0E0F_101112131415161718191A1B1C1D1E1F,00) == 0x00);
+        Assert(()=> U256.NthUint8(0x000102030405060708090A0B0C0D0E0F_101112131415161718191A1B1C1D1E1F,01) == 0x01);
+        Assert(()=> U256.NthUint8(0x000102030405060708090A0B0C0D0E0F_101112131415161718191A1B1C1D1E1F,02) == 0x02);
+        Assert(()=> U256.NthUint8(0x000102030405060708090A0B0C0D0E0F_101112131415161718191A1B1C1D1E1F,03) == 0x03);
+        Assert(()=> U256.NthUint8(0x000102030405060708090A0B0C0D0E0F_101112131415161718191A1B1C1D1E1F,04) == 0x04);
+        Assert(()=> U256.NthUint8(0x000102030405060708090A0B0C0D0E0F_101112131415161718191A1B1C1D1E1F,05) == 0x05);
+        Assert(()=> U256.NthUint8(0x000102030405060708090A0B0C0D0E0F_101112131415161718191A1B1C1D1E1F,06) == 0x06);
+        Assert(()=> U256.NthUint8(0x000102030405060708090A0B0C0D0E0F_101112131415161718191A1B1C1D1E1F,07) == 0x07);
+        Assert(()=> U256.NthUint8(0x000102030405060708090A0B0C0D0E0F_101112131415161718191A1B1C1D1E1F,08) == 0x08);
+        Assert(()=> U256.NthUint8(0x000102030405060708090A0B0C0D0E0F_101112131415161718191A1B1C1D1E1F,09) == 0x09);
+        Assert(()=> U256.NthUint8(0x000102030405060708090A0B0C0D0E0F_101112131415161718191A1B1C1D1E1F,10) == 0x0A);
+        Assert(()=> U256.NthUint8(0x000102030405060708090A0B0C0D0E0F_101112131415161718191A1B1C1D1E1F,11) == 0x0B);
+        Assert(()=> U256.NthUint8(0x000102030405060708090A0B0C0D0E0F_101112131415161718191A1B1C1D1E1F,12) == 0x0C);
+        Assert(()=> U256.NthUint8(0x000102030405060708090A0B0C0D0E0F_101112131415161718191A1B1C1D1E1F,13) == 0x0D);
+        Assert(()=> U256.NthUint8(0x000102030405060708090A0B0C0D0E0F_101112131415161718191A1B1C1D1E1F,14) == 0x0E);
+        Assert(()=> U256.NthUint8(0x000102030405060708090A0B0C0D0E0F_101112131415161718191A1B1C1D1E1F,15) == 0x0F);
+        Assert(()=> U256.NthUint8(0x000102030405060708090A0B0C0D0E0F_101112131415161718191A1B1C1D1E1F,16) == 0x10);
+        Assert(()=> U256.NthUint8(0x000102030405060708090A0B0C0D0E0F_101112131415161718191A1B1C1D1E1F,17) == 0x11);
+        Assert(()=> U256.NthUint8(0x000102030405060708090A0B0C0D0E0F_101112131415161718191A1B1C1D1E1F,18) == 0x12);
+        Assert(()=> U256.NthUint8(0x000102030405060708090A0B0C0D0E0F_101112131415161718191A1B1C1D1E1F,19) == 0x13);
+        Assert(()=> U256.NthUint8(0x000102030405060708090A0B0C0D0E0F_101112131415161718191A1B1C1D1E1F,20) == 0x14);
+        Assert(()=> U256.NthUint8(0x000102030405060708090A0B0C0D0E0F_101112131415161718191A1B1C1D1E1F,21) == 0x15);
+        Assert(()=> U256.NthUint8(0x000102030405060708090A0B0C0D0E0F_101112131415161718191A1B1C1D1E1F,22) == 0x16);
+        Assert(()=> U256.NthUint8(0x000102030405060708090A0B0C0D0E0F_101112131415161718191A1B1C1D1E1F,23) == 0x17);
+        Assert(()=> U256.NthUint8(0x000102030405060708090A0B0C0D0E0F_101112131415161718191A1B1C1D1E1F,24) == 0x18);
+        Assert(()=> U256.NthUint8(0x000102030405060708090A0B0C0D0E0F_101112131415161718191A1B1C1D1E1F,25) == 0x19);
+        Assert(()=> U256.NthUint8(0x000102030405060708090A0B0C0D0E0F_101112131415161718191A1B1C1D1E1F,26) == 0x1A);
+        Assert(()=> U256.NthUint8(0x000102030405060708090A0B0C0D0E0F_101112131415161718191A1B1C1D1E1F,27) == 0x1B);
+        Assert(()=> U256.NthUint8(0x000102030405060708090A0B0C0D0E0F_101112131415161718191A1B1C1D1E1F,28) == 0x1C);
+        Assert(()=> U256.NthUint8(0x000102030405060708090A0B0C0D0E0F_101112131415161718191A1B1C1D1E1F,29) == 0x1D);
+        Assert(()=> U256.NthUint8(0x000102030405060708090A0B0C0D0E0F_101112131415161718191A1B1C1D1E1F,30) == 0x1E);
+        Assert(()=> U256.NthUint8(0x000102030405060708090A0B0C0D0E0F_101112131415161718191A1B1C1D1E1F,31) == 0x1F);
+    }
 
-method {:test} ToBytesTests() {
-    // U16
-    Assert(()=>U16.ToBytes(0) == [0x00,0x00]);
-    Assert(()=>U16.ToBytes(1) == [0x00,0x01]);
-    Assert(()=>U16.ToBytes(258) == [0x01,0x02]);
-    Assert(()=>U16.ToBytes(32769) == [0x80,0x01]);
-    // U32
-    Assert(()=>U32.ToBytes(0) == [0x00,0x00,0x00,0x00]);
-    Assert(()=>U32.ToBytes(1) == [0x00,0x00,0x00,0x01]);
-    Assert(()=>U32.ToBytes(258) == [0x00,0x00,0x01,0x02]);
-    Assert(()=>U32.ToBytes(33554437) == [0x02,0x00,0x00,0x05]);
-    // U64
-    Assert(()=>U64.ToBytes(0) == [0x00,0x00,0x00,0x00,0x00,0x00,0x00,0x00]);
-    Assert(()=>U64.ToBytes(1) == [0x00,0x00,0x00,0x00,0x00,0x00,0x00,0x01]);
-    Assert(()=>U64.ToBytes(258) == [0x00,0x00,0x00,0x00,0x00,0x00,0x01,0x02]);
-    Assert(()=>U64.ToBytes(33554437) == [0x00,0x00,0x00,0x00,0x02,0x00,0x00,0x05]);
-    Assert(()=>U64.ToBytes(65536 * 33554437) == [0x00,0x00,0x02,0x00,0x00,0x05,0x00,0x00]);
-}
+    method {:test} ToBytesTests() {
+        // U16
+        Assert(()=>U16.ToBytes(0) == [0x00,0x00]);
+        Assert(()=>U16.ToBytes(1) == [0x00,0x01]);
+        Assert(()=>U16.ToBytes(258) == [0x01,0x02]);
+        Assert(()=>U16.ToBytes(32769) == [0x80,0x01]);
+        // U32
+        Assert(()=>U32.ToBytes(0) == [0x00,0x00,0x00,0x00]);
+        Assert(()=>U32.ToBytes(1) == [0x00,0x00,0x00,0x01]);
+        Assert(()=>U32.ToBytes(258) == [0x00,0x00,0x01,0x02]);
+        Assert(()=>U32.ToBytes(33554437) == [0x02,0x00,0x00,0x05]);
+        // U64
+        Assert(()=>U64.ToBytes(0) == [0x00,0x00,0x00,0x00,0x00,0x00,0x00,0x00]);
+        Assert(()=>U64.ToBytes(1) == [0x00,0x00,0x00,0x00,0x00,0x00,0x00,0x01]);
+        Assert(()=>U64.ToBytes(258) == [0x00,0x00,0x00,0x00,0x00,0x00,0x01,0x02]);
+        Assert(()=>U64.ToBytes(33554437) == [0x00,0x00,0x00,0x00,0x02,0x00,0x00,0x05]);
+        Assert(()=>U64.ToBytes(65536 * 33554437) == [0x00,0x00,0x02,0x00,0x00,0x05,0x00,0x00]);
+    }
 
-method {:test} SarTests() {
-    Assert(()=>I256.Sar(4, 1) == 2);
-    Assert(()=>I256.Sar(4, 2) == 1);
-    Assert(()=>I256.Sar(4, 3) == 0);
-    Assert(()=>I256.Sar(4, 4) == 0);
-    Assert(()=>I256.Sar(15, 1) == 7);
-    Assert(()=>I256.Sar(15, 2) == 3);
-    Assert(()=>I256.Sar(15, 3) == 1);
-    Assert(()=>I256.Sar(15, 4) == 0);
-    Assert(()=>I256.Sar(90, 1) == 45);
-    Assert(()=>I256.Sar(90, 2) == 22);
-    Assert(()=>I256.Sar(90, 3) == 11);
-    Assert(()=>I256.Sar(90, 4) == 5);
-    Assert(()=>I256.Sar(-90, 1) == -45);
-    Assert(()=>I256.Sar(-90, 2) == -23);
-    Assert(()=>I256.Sar(-90, 3) == -12);
-    Assert(()=>I256.Sar(-90, 4) == -6);
-    Assert(()=>I256.Sar(-15, 1) == -8);
-    Assert(()=>I256.Sar(-15, 2) == -4);
-    Assert(()=>I256.Sar(-15, 3) == -2);
-    Assert(()=>I256.Sar(-15, 4) == -1);
-    Assert(()=>I256.Sar(-4, 1) == -2);
-    Assert(()=>I256.Sar(-4, 2) == -1);
-    Assert(()=>I256.Sar(-4, 3) == -1);
-    Assert(()=>I256.Sar(-4, 4) == -1);
-    Assert(()=>I256.Sar(-1, 1) == -1);
-    Assert(()=>I256.Sar(1, 256) == 0);
-    Assert(()=>I256.Sar(-1, 256) == -1);
-    Assert(()=>I256.Sar(-TWO_128 as i256, 256) == -1);
-}
+    method {:test} SarTests() {
+        Assert(()=>I256.Sar(4, 1) == 2);
+        Assert(()=>I256.Sar(4, 2) == 1);
+        Assert(()=>I256.Sar(4, 3) == 0);
+        Assert(()=>I256.Sar(4, 4) == 0);
+        Assert(()=>I256.Sar(15, 1) == 7);
+        Assert(()=>I256.Sar(15, 2) == 3);
+        Assert(()=>I256.Sar(15, 3) == 1);
+        Assert(()=>I256.Sar(15, 4) == 0);
+        Assert(()=>I256.Sar(90, 1) == 45);
+        Assert(()=>I256.Sar(90, 2) == 22);
+        Assert(()=>I256.Sar(90, 3) == 11);
+        Assert(()=>I256.Sar(90, 4) == 5);
+        Assert(()=>I256.Sar(-90, 1) == -45);
+        Assert(()=>I256.Sar(-90, 2) == -23);
+        Assert(()=>I256.Sar(-90, 3) == -12);
+        Assert(()=>I256.Sar(-90, 4) == -6);
+        Assert(()=>I256.Sar(-15, 1) == -8);
+        Assert(()=>I256.Sar(-15, 2) == -4);
+        Assert(()=>I256.Sar(-15, 3) == -2);
+        Assert(()=>I256.Sar(-15, 4) == -1);
+        Assert(()=>I256.Sar(-4, 1) == -2);
+        Assert(()=>I256.Sar(-4, 2) == -1);
+        Assert(()=>I256.Sar(-4, 3) == -1);
+        Assert(()=>I256.Sar(-4, 4) == -1);
+        Assert(()=>I256.Sar(-1, 1) == -1);
+        Assert(()=>I256.Sar(1, 256) == 0);
+        Assert(()=>I256.Sar(-1, 256) == -1);
+        Assert(()=>I256.Sar(-TWO_128 as i256, 256) == -1);
+    }
 
-method {:test} Log2Tests() {
-    // U8
-    Assert(()=> U8.Log2(0) == 0);
-    Assert(()=> U8.Log2(1) == 0);
-    Assert(()=> U8.Log2(2) == 1);
-    Assert(()=> U8.Log2(3) == 1);
-    Assert(()=> U8.Log2(4) == 2);
-    Assert(()=> U8.Log2(5) == 2);
-    Assert(()=> U8.Log2(6) == 2);
-    Assert(()=> U8.Log2(7) == 2);
-    Assert(()=> U8.Log2(8) == 3);
-    Assert(()=> U8.Log2(9) == 3);
-    Assert(()=> U8.Log2(10) == 3);
-    Assert(()=> U8.Log2(11) == 3);
-    Assert(()=> U8.Log2(12) == 3);
-    Assert(()=> U8.Log2(13) == 3);
-    Assert(()=> U8.Log2(14) == 3);
-    Assert(()=> U8.Log2(15) == 3);
-    Assert(()=> U8.Log2(16) == 4);
-    Assert(()=> U8.Log2(17) == 4);
-    Assert(()=> U8.Log2(28) == 4);
-    Assert(()=> U8.Log2(29) == 4);
-    Assert(()=> U8.Log2(30) == 4);
-    Assert(()=> U8.Log2(31) == 4);
-    Assert(()=> U8.Log2(32) == 5);
-    Assert(()=> U8.Log2(33) == 5);
-    Assert(()=> U8.Log2(60) == 5);
-    Assert(()=> U8.Log2(61) == 5);
-    Assert(()=> U8.Log2(62) == 5);
-    Assert(()=> U8.Log2(63) == 5);
-    Assert(()=> U8.Log2(64) == 6);
-    Assert(()=> U8.Log2(65) == 6);
-    Assert(()=> U8.Log2(66) == 6);
-    Assert(()=> U8.Log2(126) == 6);
-    Assert(()=> U8.Log2(127) == 6);
-    Assert(()=> U8.Log2(128) == 7);
-    Assert(()=> U8.Log2(129) == 7);
-    Assert(()=> U8.Log2(130) == 7);
-    Assert(()=> U8.Log2(181) == 7);
-    Assert(()=> U8.Log2(182) == 7);
-    Assert(()=> U8.Log2(183) == 7);
-    Assert(()=> U8.Log2(184) == 7);
-    Assert(()=> U8.Log2(185) == 7);
-    Assert(()=> U8.Log2(186) == 7);
-    Assert(()=> U8.Log2(254) == 7);
-    Assert(()=> U8.Log2(255) == 7);
-    // U16
-    Assert(()=> U16.Log2(0) == 0);
-    Assert(()=> U16.Log2(1) == 0);
-    Assert(()=> U16.Log2(2) == 1);
-    Assert(()=> U16.Log2(3) == 1);
-    Assert(()=> U16.Log2(4) == 2);
-    Assert(()=> U16.Log2(5) == 2);
-    Assert(()=> U16.Log2(254) == 7);
-    Assert(()=> U16.Log2(255) == 7);
-    Assert(()=> U16.Log2(256) == 8);
-    Assert(()=> U16.Log2(257) == 8);
-    Assert(()=> U16.Log2(511) == 8);
-    Assert(()=> U16.Log2(512) == 9);
-    Assert(()=> U16.Log2(513) == 9);
-    Assert(()=> U16.Log2(1023) == 9);
-    Assert(()=> U16.Log2(1024) == 10);
-    Assert(()=> U16.Log2(1025) == 10);
-    Assert(()=> U16.Log2(65534) == 15);
-    Assert(()=> U16.Log2(65535) == 15);
-    // U32
-    Assert(()=> U32.Log2(0) == 0);
-    Assert(()=> U32.Log2(1) == 0);
-    Assert(()=> U32.Log2(2) == 1);
-    Assert(()=> U32.Log2(3) == 1);
-    Assert(()=> U32.Log2(4) == 2);
-    Assert(()=> U32.Log2(5) == 2);
-    Assert(()=> U32.Log2(254) == 7);
-    Assert(()=> U32.Log2(255) == 7);
-    Assert(()=> U32.Log2(65535) == 15);
-    Assert(()=> U32.Log2(65536) == 16);
-    Assert(()=> U32.Log2(131071) == 16);
-    Assert(()=> U32.Log2(131072) == 17);
-    Assert(()=> U32.Log2(262143) == 17);
-    Assert(()=> U32.Log2(262144) == 18);
-    Assert(()=> U32.Log2(MAX_U32 as u32) == 31);
-    // U64
-    Assert(()=> U64.Log2(0) == 0);
-    Assert(()=> U64.Log2(1) == 0);
-    Assert(()=> U64.Log2(2) == 1);
-    Assert(()=> U64.Log2(3) == 1);
-    Assert(()=> U64.Log2(4) == 2);
-    Assert(()=> U64.Log2(5) == 2);
-    Assert(()=> U64.Log2(254) == 7);
-    Assert(()=> U64.Log2(255) == 7);
-    Assert(()=> U64.Log2(65535) == 15);
-    Assert(()=> U64.Log2(65536) == 16);
-    Assert(()=> U64.Log2(MAX_U32 as u64) == 31);
-    Assert(()=> U64.Log2(TWO_32 as u64) == 32);
-    Assert(()=> U64.Log2(MAX_U64 as u64) == 63);
-    // U128
-    Assert(()=> U128.Log2(0) == 0);
-    Assert(()=> U128.Log2(1) == 0);
-    Assert(()=> U128.Log2(2) == 1);
-    Assert(()=> U128.Log2(3) == 1);
-    Assert(()=> U128.Log2(4) == 2);
-    Assert(()=> U128.Log2(5) == 2);
-    Assert(()=> U128.Log2(254) == 7);
-    Assert(()=> U128.Log2(255) == 7);
-    Assert(()=> U128.Log2(65535) == 15);
-    Assert(()=> U128.Log2(65536) == 16);
-    Assert(()=> U128.Log2(MAX_U32 as u128) == 31);
-    Assert(()=> U128.Log2(TWO_32 as u128) == 32);
-    Assert(()=> U128.Log2(MAX_U64 as u128) == 63);
-    Assert(()=> U128.Log2(TWO_64 as u128) == 64);
-    Assert(()=> U128.Log2(MAX_U128 as u128) == 127);
-    // U256
-    Assert(()=> U256.Log2(0) == 0);
-    Assert(()=> U256.Log2(1) == 0);
-    Assert(()=> U256.Log2(2) == 1);
-    Assert(()=> U256.Log2(3) == 1);
-    Assert(()=> U256.Log2(4) == 2);
-    Assert(()=> U256.Log2(5) == 2);
-    Assert(()=> U256.Log2(254) == 7);
-    Assert(()=> U256.Log2(255) == 7);
-    Assert(()=> U256.Log2(65535) == 15);
-    Assert(()=> U256.Log2(65536) == 16);
-    Assert(()=> U256.Log2(MAX_U32 as u256) == 31);
-    Assert(()=> U256.Log2(TWO_32 as u256) == 32);
-    Assert(()=> U256.Log2(MAX_U64 as u256) == 63);
-    Assert(()=> U256.Log2(TWO_64 as u256) == 64);
-    Assert(()=> U256.Log2(MAX_U128 as u256) == 127);
-    Assert(()=> U256.Log2(TWO_128 as u256) == 128);
-    Assert(()=> U256.Log2(MAX_U256 as u256) == 255);
-}
+    method {:test} Log2Tests() {
+        // U8
+        Assert(()=> U8.Log2(0) == 0);
+        Assert(()=> U8.Log2(1) == 0);
+        Assert(()=> U8.Log2(2) == 1);
+        Assert(()=> U8.Log2(3) == 1);
+        Assert(()=> U8.Log2(4) == 2);
+        Assert(()=> U8.Log2(5) == 2);
+        Assert(()=> U8.Log2(6) == 2);
+        Assert(()=> U8.Log2(7) == 2);
+        Assert(()=> U8.Log2(8) == 3);
+        Assert(()=> U8.Log2(9) == 3);
+        Assert(()=> U8.Log2(10) == 3);
+        Assert(()=> U8.Log2(11) == 3);
+        Assert(()=> U8.Log2(12) == 3);
+        Assert(()=> U8.Log2(13) == 3);
+        Assert(()=> U8.Log2(14) == 3);
+        Assert(()=> U8.Log2(15) == 3);
+        Assert(()=> U8.Log2(16) == 4);
+        Assert(()=> U8.Log2(17) == 4);
+        Assert(()=> U8.Log2(28) == 4);
+        Assert(()=> U8.Log2(29) == 4);
+        Assert(()=> U8.Log2(30) == 4);
+        Assert(()=> U8.Log2(31) == 4);
+        Assert(()=> U8.Log2(32) == 5);
+        Assert(()=> U8.Log2(33) == 5);
+        Assert(()=> U8.Log2(60) == 5);
+        Assert(()=> U8.Log2(61) == 5);
+        Assert(()=> U8.Log2(62) == 5);
+        Assert(()=> U8.Log2(63) == 5);
+        Assert(()=> U8.Log2(64) == 6);
+        Assert(()=> U8.Log2(65) == 6);
+        Assert(()=> U8.Log2(66) == 6);
+        Assert(()=> U8.Log2(126) == 6);
+        Assert(()=> U8.Log2(127) == 6);
+        Assert(()=> U8.Log2(128) == 7);
+        Assert(()=> U8.Log2(129) == 7);
+        Assert(()=> U8.Log2(130) == 7);
+        Assert(()=> U8.Log2(181) == 7);
+        Assert(()=> U8.Log2(182) == 7);
+        Assert(()=> U8.Log2(183) == 7);
+        Assert(()=> U8.Log2(184) == 7);
+        Assert(()=> U8.Log2(185) == 7);
+        Assert(()=> U8.Log2(186) == 7);
+        Assert(()=> U8.Log2(254) == 7);
+        Assert(()=> U8.Log2(255) == 7);
+        // U16
+        Assert(()=> U16.Log2(0) == 0);
+        Assert(()=> U16.Log2(1) == 0);
+        Assert(()=> U16.Log2(2) == 1);
+        Assert(()=> U16.Log2(3) == 1);
+        Assert(()=> U16.Log2(4) == 2);
+        Assert(()=> U16.Log2(5) == 2);
+        Assert(()=> U16.Log2(254) == 7);
+        Assert(()=> U16.Log2(255) == 7);
+        Assert(()=> U16.Log2(256) == 8);
+        Assert(()=> U16.Log2(257) == 8);
+        Assert(()=> U16.Log2(511) == 8);
+        Assert(()=> U16.Log2(512) == 9);
+        Assert(()=> U16.Log2(513) == 9);
+        Assert(()=> U16.Log2(1023) == 9);
+        Assert(()=> U16.Log2(1024) == 10);
+        Assert(()=> U16.Log2(1025) == 10);
+        Assert(()=> U16.Log2(65534) == 15);
+        Assert(()=> U16.Log2(65535) == 15);
+        // U32
+        Assert(()=> U32.Log2(0) == 0);
+        Assert(()=> U32.Log2(1) == 0);
+        Assert(()=> U32.Log2(2) == 1);
+        Assert(()=> U32.Log2(3) == 1);
+        Assert(()=> U32.Log2(4) == 2);
+        Assert(()=> U32.Log2(5) == 2);
+        Assert(()=> U32.Log2(254) == 7);
+        Assert(()=> U32.Log2(255) == 7);
+        Assert(()=> U32.Log2(65535) == 15);
+        Assert(()=> U32.Log2(65536) == 16);
+        Assert(()=> U32.Log2(131071) == 16);
+        Assert(()=> U32.Log2(131072) == 17);
+        Assert(()=> U32.Log2(262143) == 17);
+        Assert(()=> U32.Log2(262144) == 18);
+        Assert(()=> U32.Log2(MAX_U32 as u32) == 31);
+        // U64
+        Assert(()=> U64.Log2(0) == 0);
+        Assert(()=> U64.Log2(1) == 0);
+        Assert(()=> U64.Log2(2) == 1);
+        Assert(()=> U64.Log2(3) == 1);
+        Assert(()=> U64.Log2(4) == 2);
+        Assert(()=> U64.Log2(5) == 2);
+        Assert(()=> U64.Log2(254) == 7);
+        Assert(()=> U64.Log2(255) == 7);
+        Assert(()=> U64.Log2(65535) == 15);
+        Assert(()=> U64.Log2(65536) == 16);
+        Assert(()=> U64.Log2(MAX_U32 as u64) == 31);
+        Assert(()=> U64.Log2(TWO_32 as u64) == 32);
+        Assert(()=> U64.Log2(MAX_U64 as u64) == 63);
+        // U128
+        Assert(()=> U128.Log2(0) == 0);
+        Assert(()=> U128.Log2(1) == 0);
+        Assert(()=> U128.Log2(2) == 1);
+        Assert(()=> U128.Log2(3) == 1);
+        Assert(()=> U128.Log2(4) == 2);
+        Assert(()=> U128.Log2(5) == 2);
+        Assert(()=> U128.Log2(254) == 7);
+        Assert(()=> U128.Log2(255) == 7);
+        Assert(()=> U128.Log2(65535) == 15);
+        Assert(()=> U128.Log2(65536) == 16);
+        Assert(()=> U128.Log2(MAX_U32 as u128) == 31);
+        Assert(()=> U128.Log2(TWO_32 as u128) == 32);
+        Assert(()=> U128.Log2(MAX_U64 as u128) == 63);
+        Assert(()=> U128.Log2(TWO_64 as u128) == 64);
+        Assert(()=> U128.Log2(MAX_U128 as u128) == 127);
+        // U256
+        Assert(()=> U256.Log2(0) == 0);
+        Assert(()=> U256.Log2(1) == 0);
+        Assert(()=> U256.Log2(2) == 1);
+        Assert(()=> U256.Log2(3) == 1);
+        Assert(()=> U256.Log2(4) == 2);
+        Assert(()=> U256.Log2(5) == 2);
+        Assert(()=> U256.Log2(254) == 7);
+        Assert(()=> U256.Log2(255) == 7);
+        Assert(()=> U256.Log2(65535) == 15);
+        Assert(()=> U256.Log2(65536) == 16);
+        Assert(()=> U256.Log2(MAX_U32 as u256) == 31);
+        Assert(()=> U256.Log2(TWO_32 as u256) == 32);
+        Assert(()=> U256.Log2(MAX_U64 as u256) == 63);
+        Assert(()=> U256.Log2(TWO_64 as u256) == 64);
+        Assert(()=> U256.Log2(MAX_U128 as u256) == 127);
+        Assert(()=> U256.Log2(TWO_128 as u256) == 128);
+        Assert(()=> U256.Log2(MAX_U256 as u256) == 255);
+    }
 
-method {:test} Log256Tests() {
-    Assert(()=> U256.Log256(0) == 0);
-    Assert(()=> U256.Log256(1) == 0);
-    Assert(()=> U256.Log256(0x80) == 0);
-    Assert(()=> U256.Log256(0xff) == 0);
-    Assert(()=> U256.Log256(0x100) == 1);
-    Assert(()=> U256.Log256(0x554) == 1);
-    Assert(()=> U256.Log256(0x3334) == 1);
-    Assert(()=> U256.Log256(0xffff) == 1);
-    Assert(()=> U256.Log256(0x1_0000) == 2);
-    Assert(()=> U256.Log256(1020314) == 2);
-    Assert(()=> U256.Log256(16777215) == 2);
-    Assert(()=> U256.Log256(16777216) == 3);
-    Assert(()=> U256.Log256(1677091272) == 3);
-    Assert(()=> U256.Log256(0xffff_ffff) == 3);
-    Assert(()=> U256.Log256(0x1_0000_0000) == 4);
-    Assert(()=> U256.Log256(0xffff_ffff_ff) == 4);
-    Assert(()=> U256.Log256(0x1_0000_0000_00) == 5);
-    Assert(()=> U256.Log256(0xffff_ffff_ffff) == 5);
-    Assert(()=> U256.Log256(0x1_0000_0000_0000) == 6);
-    Assert(()=> U256.Log256(0xffff_ffff_ffff_ff) == 6);
-    Assert(()=> U256.Log256(0x1_0000_0000_0000_00) == 7);
-    Assert(()=> U256.Log256(0xffff_ffff_ffff_ffff) == 7);
-    Assert(()=> U256.Log256(0x1_0000_0000_0000_0000) == 8);
-    Assert(()=> U256.Log256(0xffff_ffff_ffff_ffff_ff) == 8);
-    Assert(()=> U256.Log256(0x1_0000_0000_0000_0000_00) == 9);
-    Assert(()=> U256.Log256(0xffff_ffff_ffff_ffff_ffff) == 9);
-    Assert(()=> U256.Log256(0x1_0000_0000_0000_0000_0000) == 10);
-    Assert(()=> U256.Log256(0xffff_ffff_ffff_ffff_ffff_ff) == 10);
-    Assert(()=> U256.Log256(0x1_0000_0000_0000_0000_0000_00) == 11);
-    Assert(()=> U256.Log256(0xffff_ffff_ffff_ffff_ffff_ffff) == 11);
-    Assert(()=> U256.Log256(0x1_0000_0000_0000_0000_0000_0000) == 12);
-    Assert(()=> U256.Log256(0xffff_ffff_ffff_ffff_ffff_ffff_ff) == 12);
-    Assert(()=> U256.Log256(0x1_0000_0000_0000_0000_0000_0000_00) == 13);
-    Assert(()=> U256.Log256(0xffff_ffff_ffff_ffff_ffff_ffff_ffff) == 13);
-    Assert(()=> U256.Log256(0x1_0000_0000_0000_0000_0000_0000_0000) == 14);
-    Assert(()=> U256.Log256(0xffff_ffff_ffff_ffff_ffff_ffff_ffff_ff) == 14);
-    Assert(()=> U256.Log256(0x1_0000_0000_0000_0000_0000_0000_0000_00) == 15);
-    Assert(()=> U256.Log256(0xffff_ffff_ffff_ffff_ffff_ffff_ffff_ffff) == 15);
-    Assert(()=> U256.Log256(0x1_0000_0000_0000_0000_0000_0000_0000_0000) == 16);
-    Assert(()=> U256.Log256(0xffff_ffff_ffff_ffff_ffff_ffff_ffff_ffff_ff) == 16);
-    Assert(()=> U256.Log256(0x1_0000_0000_0000_0000_0000_0000_0000_0000_00) == 17);
-    Assert(()=> U256.Log256(0xffff_ffff_ffff_ffff_ffff_ffff_ffff_ffff_ffff) == 17);
-    Assert(()=> U256.Log256(0x1_0000_0000_0000_0000_0000_0000_0000_0000_0000) == 18);
-    Assert(()=> U256.Log256(0xffff_ffff_ffff_ffff_ffff_ffff_ffff_ffff_ffff_ff) == 18);
-    Assert(()=> U256.Log256(0x1_0000_0000_0000_0000_0000_0000_0000_0000_0000_00) == 19);
-    Assert(()=> U256.Log256(0xffff_ffff_ffff_ffff_ffff_ffff_ffff_ffff_ffff_ffff) == 19);
-    Assert(()=> U256.Log256(0x1_0000_0000_0000_0000_0000_0000_0000_0000_0000_0000) == 20);
-    Assert(()=> U256.Log256(0xffff_ffff_ffff_ffff_ffff_ffff_ffff_ffff_ffff_ffff_ff) == 20);
-    Assert(()=> U256.Log256(0x1_0000_0000_0000_0000_0000_0000_0000_0000_0000_0000_00) == 21);
-    Assert(()=> U256.Log256(0xffff_ffff_ffff_ffff_ffff_ffff_ffff_ffff_ffff_ffff_ffff) == 21);
-    Assert(()=> U256.Log256(0x1_0000_0000_0000_0000_0000_0000_0000_0000_0000_0000_0000) == 22);
-    Assert(()=> U256.Log256(0xffff_ffff_ffff_ffff_ffff_ffff_ffff_ffff_ffff_ffff_ffff_ff) == 22);
-    Assert(()=> U256.Log256(0x1_0000_0000_0000_0000_0000_0000_0000_0000_0000_0000_0000_00) == 23);
-    Assert(()=> U256.Log256(0xffff_ffff_ffff_ffff_ffff_ffff_ffff_ffff_ffff_ffff_ffff_ffff) == 23);
-    Assert(()=> U256.Log256(0x1_0000_0000_0000_0000_0000_0000_0000_0000_0000_0000_0000_0000) == 24);
-    Assert(()=> U256.Log256(0xffff_ffff_ffff_ffff_ffff_ffff_ffff_ffff_ffff_ffff_ffff_ffff_ff) == 24);
-    Assert(()=> U256.Log256(0x1_0000_0000_0000_0000_0000_0000_0000_0000_0000_0000_0000_0000_00) == 25);
-    Assert(()=> U256.Log256(0xffff_ffff_ffff_ffff_ffff_ffff_ffff_ffff_ffff_ffff_ffff_ffff_ffff) == 25);
-    Assert(()=> U256.Log256(0x1_0000_0000_0000_0000_0000_0000_0000_0000_0000_0000_0000_0000_0000) == 26);
-    Assert(()=> U256.Log256(0xffff_ffff_ffff_ffff_ffff_ffff_ffff_ffff_ffff_ffff_ffff_ffff_ffff_ff) == 26);
-    Assert(()=> U256.Log256(0x1_0000_0000_0000_0000_0000_0000_0000_0000_0000_0000_0000_0000_0000_00) == 27);
-    Assert(()=> U256.Log256(0xffff_ffff_ffff_ffff_ffff_ffff_ffff_ffff_ffff_ffff_ffff_ffff_ffff_ffff) == 27);
-    Assert(()=> U256.Log256(0x1_0000_0000_0000_0000_0000_0000_0000_0000_0000_0000_0000_0000_0000_0000) == 28);
-    Assert(()=> U256.Log256(0xffff_ffff_ffff_ffff_ffff_ffff_ffff_ffff_ffff_ffff_ffff_ffff_ffff_ffff_ff) == 28);
-    Assert(()=> U256.Log256(0x1_0000_0000_0000_0000_0000_0000_0000_0000_0000_0000_0000_0000_0000_0000_00) == 29);
-    Assert(()=> U256.Log256(0xffff_ffff_ffff_ffff_ffff_ffff_ffff_ffff_ffff_ffff_ffff_ffff_ffff_ffff_ffff) == 29);
-    Assert(()=> U256.Log256(0x1_0000_0000_0000_0000_0000_0000_0000_0000_0000_0000_0000_0000_0000_0000_0000) == 30);
-    Assert(()=> U256.Log256(0xffff_ffff_ffff_ffff_ffff_ffff_ffff_ffff_ffff_ffff_ffff_ffff_ffff_ffff_ffff_ff) == 30);
-    Assert(()=> U256.Log256(0x1_0000_0000_0000_0000_0000_0000_0000_0000_0000_0000_0000_0000_0000_0000_0000_00) == 31);
-    Assert(()=> U256.Log256(0xffff_ffff_ffff_ffff_ffff_ffff_ffff_ffff_ffff_ffff_ffff_ffff_ffff_ffff_ffff_ffff) == 31);
-}
+    method {:test} Log256Tests() {
+        Assert(()=> U256.Log256(0) == 0);
+        Assert(()=> U256.Log256(1) == 0);
+        Assert(()=> U256.Log256(0x80) == 0);
+        Assert(()=> U256.Log256(0xff) == 0);
+        Assert(()=> U256.Log256(0x100) == 1);
+        Assert(()=> U256.Log256(0x554) == 1);
+        Assert(()=> U256.Log256(0x3334) == 1);
+        Assert(()=> U256.Log256(0xffff) == 1);
+        Assert(()=> U256.Log256(0x1_0000) == 2);
+        Assert(()=> U256.Log256(1020314) == 2);
+        Assert(()=> U256.Log256(16777215) == 2);
+        Assert(()=> U256.Log256(16777216) == 3);
+        Assert(()=> U256.Log256(1677091272) == 3);
+        Assert(()=> U256.Log256(0xffff_ffff) == 3);
+        Assert(()=> U256.Log256(0x1_0000_0000) == 4);
+        Assert(()=> U256.Log256(0xffff_ffff_ff) == 4);
+        Assert(()=> U256.Log256(0x1_0000_0000_00) == 5);
+        Assert(()=> U256.Log256(0xffff_ffff_ffff) == 5);
+        Assert(()=> U256.Log256(0x1_0000_0000_0000) == 6);
+        Assert(()=> U256.Log256(0xffff_ffff_ffff_ff) == 6);
+        Assert(()=> U256.Log256(0x1_0000_0000_0000_00) == 7);
+        Assert(()=> U256.Log256(0xffff_ffff_ffff_ffff) == 7);
+        Assert(()=> U256.Log256(0x1_0000_0000_0000_0000) == 8);
+        Assert(()=> U256.Log256(0xffff_ffff_ffff_ffff_ff) == 8);
+        Assert(()=> U256.Log256(0x1_0000_0000_0000_0000_00) == 9);
+        Assert(()=> U256.Log256(0xffff_ffff_ffff_ffff_ffff) == 9);
+        Assert(()=> U256.Log256(0x1_0000_0000_0000_0000_0000) == 10);
+        Assert(()=> U256.Log256(0xffff_ffff_ffff_ffff_ffff_ff) == 10);
+        Assert(()=> U256.Log256(0x1_0000_0000_0000_0000_0000_00) == 11);
+        Assert(()=> U256.Log256(0xffff_ffff_ffff_ffff_ffff_ffff) == 11);
+        Assert(()=> U256.Log256(0x1_0000_0000_0000_0000_0000_0000) == 12);
+        Assert(()=> U256.Log256(0xffff_ffff_ffff_ffff_ffff_ffff_ff) == 12);
+        Assert(()=> U256.Log256(0x1_0000_0000_0000_0000_0000_0000_00) == 13);
+        Assert(()=> U256.Log256(0xffff_ffff_ffff_ffff_ffff_ffff_ffff) == 13);
+        Assert(()=> U256.Log256(0x1_0000_0000_0000_0000_0000_0000_0000) == 14);
+        Assert(()=> U256.Log256(0xffff_ffff_ffff_ffff_ffff_ffff_ffff_ff) == 14);
+        Assert(()=> U256.Log256(0x1_0000_0000_0000_0000_0000_0000_0000_00) == 15);
+        Assert(()=> U256.Log256(0xffff_ffff_ffff_ffff_ffff_ffff_ffff_ffff) == 15);
+        Assert(()=> U256.Log256(0x1_0000_0000_0000_0000_0000_0000_0000_0000) == 16);
+        Assert(()=> U256.Log256(0xffff_ffff_ffff_ffff_ffff_ffff_ffff_ffff_ff) == 16);
+        Assert(()=> U256.Log256(0x1_0000_0000_0000_0000_0000_0000_0000_0000_00) == 17);
+        Assert(()=> U256.Log256(0xffff_ffff_ffff_ffff_ffff_ffff_ffff_ffff_ffff) == 17);
+        Assert(()=> U256.Log256(0x1_0000_0000_0000_0000_0000_0000_0000_0000_0000) == 18);
+        Assert(()=> U256.Log256(0xffff_ffff_ffff_ffff_ffff_ffff_ffff_ffff_ffff_ff) == 18);
+        Assert(()=> U256.Log256(0x1_0000_0000_0000_0000_0000_0000_0000_0000_0000_00) == 19);
+        Assert(()=> U256.Log256(0xffff_ffff_ffff_ffff_ffff_ffff_ffff_ffff_ffff_ffff) == 19);
+        Assert(()=> U256.Log256(0x1_0000_0000_0000_0000_0000_0000_0000_0000_0000_0000) == 20);
+        Assert(()=> U256.Log256(0xffff_ffff_ffff_ffff_ffff_ffff_ffff_ffff_ffff_ffff_ff) == 20);
+        Assert(()=> U256.Log256(0x1_0000_0000_0000_0000_0000_0000_0000_0000_0000_0000_00) == 21);
+        Assert(()=> U256.Log256(0xffff_ffff_ffff_ffff_ffff_ffff_ffff_ffff_ffff_ffff_ffff) == 21);
+        Assert(()=> U256.Log256(0x1_0000_0000_0000_0000_0000_0000_0000_0000_0000_0000_0000) == 22);
+        Assert(()=> U256.Log256(0xffff_ffff_ffff_ffff_ffff_ffff_ffff_ffff_ffff_ffff_ffff_ff) == 22);
+        Assert(()=> U256.Log256(0x1_0000_0000_0000_0000_0000_0000_0000_0000_0000_0000_0000_00) == 23);
+        Assert(()=> U256.Log256(0xffff_ffff_ffff_ffff_ffff_ffff_ffff_ffff_ffff_ffff_ffff_ffff) == 23);
+        Assert(()=> U256.Log256(0x1_0000_0000_0000_0000_0000_0000_0000_0000_0000_0000_0000_0000) == 24);
+        Assert(()=> U256.Log256(0xffff_ffff_ffff_ffff_ffff_ffff_ffff_ffff_ffff_ffff_ffff_ffff_ff) == 24);
+        Assert(()=> U256.Log256(0x1_0000_0000_0000_0000_0000_0000_0000_0000_0000_0000_0000_0000_00) == 25);
+        Assert(()=> U256.Log256(0xffff_ffff_ffff_ffff_ffff_ffff_ffff_ffff_ffff_ffff_ffff_ffff_ffff) == 25);
+        Assert(()=> U256.Log256(0x1_0000_0000_0000_0000_0000_0000_0000_0000_0000_0000_0000_0000_0000) == 26);
+        Assert(()=> U256.Log256(0xffff_ffff_ffff_ffff_ffff_ffff_ffff_ffff_ffff_ffff_ffff_ffff_ffff_ff) == 26);
+        Assert(()=> U256.Log256(0x1_0000_0000_0000_0000_0000_0000_0000_0000_0000_0000_0000_0000_0000_00) == 27);
+        Assert(()=> U256.Log256(0xffff_ffff_ffff_ffff_ffff_ffff_ffff_ffff_ffff_ffff_ffff_ffff_ffff_ffff) == 27);
+        Assert(()=> U256.Log256(0x1_0000_0000_0000_0000_0000_0000_0000_0000_0000_0000_0000_0000_0000_0000) == 28);
+        Assert(()=> U256.Log256(0xffff_ffff_ffff_ffff_ffff_ffff_ffff_ffff_ffff_ffff_ffff_ffff_ffff_ffff_ff) == 28);
+        Assert(()=> U256.Log256(0x1_0000_0000_0000_0000_0000_0000_0000_0000_0000_0000_0000_0000_0000_0000_00) == 29);
+        Assert(()=> U256.Log256(0xffff_ffff_ffff_ffff_ffff_ffff_ffff_ffff_ffff_ffff_ffff_ffff_ffff_ffff_ffff) == 29);
+        Assert(()=> U256.Log256(0x1_0000_0000_0000_0000_0000_0000_0000_0000_0000_0000_0000_0000_0000_0000_0000) == 30);
+        Assert(()=> U256.Log256(0xffff_ffff_ffff_ffff_ffff_ffff_ffff_ffff_ffff_ffff_ffff_ffff_ffff_ffff_ffff_ff) == 30);
+        Assert(()=> U256.Log256(0x1_0000_0000_0000_0000_0000_0000_0000_0000_0000_0000_0000_0000_0000_0000_0000_00) == 31);
+        Assert(()=> U256.Log256(0xffff_ffff_ffff_ffff_ffff_ffff_ffff_ffff_ffff_ffff_ffff_ffff_ffff_ffff_ffff_ffff) == 31);
+    }
 
-method {:test} WordTests() {
-    // ==>
-    Assert(()=> Word.asI256(0) == 0);
-    Assert(()=> Word.asI256(MAX_U256 as u256) == -1);
-    Assert(()=> Word.asI256(MAX_I256 as u256) == (MAX_I256 as i256));
-    Assert(()=> Word.asI256((MAX_I256 + 1) as u256) == (MIN_I256 as i256));
-    // <==
-    Assert(()=> Word.fromI256(0) == 0);
-    Assert(()=> Word.fromI256(-1) == (MAX_U256 as u256));
-    Assert(()=> Word.fromI256(MAX_I256 as i256) == (MAX_I256 as u256));
-    Assert(()=> Word.fromI256(MIN_I256 as i256) == (TWO_255 as u256));
+    method {:test} WordTests() {
+        // ==>
+        Assert(()=> Word.asI256(0) == 0);
+        Assert(()=> Word.asI256(MAX_U256 as u256) == -1);
+        Assert(()=> Word.asI256(MAX_I256 as u256) == (MAX_I256 as i256));
+        Assert(()=> Word.asI256((MAX_I256 + 1) as u256) == (MIN_I256 as i256));
+        // <==
+        Assert(()=> Word.fromI256(0) == 0);
+        Assert(()=> Word.fromI256(-1) == (MAX_U256 as u256));
+        Assert(()=> Word.fromI256(MAX_I256 as i256) == (MAX_I256 as u256));
+        Assert(()=> Word.fromI256(MIN_I256 as i256) == (TWO_255 as u256));
+    }
 }
